ref_impl/src/verifier/fstar_files/test_axiomatization.fst
@@ -1,0 +1,10 @@
+module Test_axiomatization
+
+open List
+open BosqueTypes
+open BosqueTerms
+open BosqueCollections
+
+val m_length : (p : bosqueTerm -> bool) -> ty:bosqueType -> x:bosqueTerm{isList ty x} -> Tot nat
+let m_length p ty x = match x with 
+| BList _ l -> (lengthList l) - (lengthList (filterList p l))
