ref_impl/src/verifier/fstar_files/trigger_example/trigger_example.fst
@@ -1,0 +1,14 @@
+module Trigger_example
+
+open Trigger_lib
+
+val positive_fun : x : list 'a -> Tot nat
+let positive_fun x = length x
+
+val another_positive_fun : x : list nat -> Tot nat
+let another_positive_fun x = length x - (length (filter (fun (x : nat) -> x = 0) x))
+
+val hmm : p : ('a -> bool) -> x : list 'a -> y : list 'a -> Lemma 
+  (requires True)
+  (ensures (length (filter p (append x y))) == (length (filter p x)) + (length (filter p y)))
+let hmm _ _ _ = ()
